Lp2lc/Active/STLC/STLCProving.lean
@@ -1,0 +1,78 @@
+-- import Std
+-- import «Lp2lc».Active.Shared
+-- import «Lp2lc».Active.Util
+-- import «Lp2lc».Active.STLC.STLCDef
+
+-- namespace Lp2lc.Active
+
+-- namespace STLC
+-- open Lp2lc.Active.Util
+
+-- section variable {I : Free}
+
+-- structure TrmIn where
+--   self: AST.Trm I
+--   fuel: Nat
+
+-- def isSafe -- doesn't use type
+--   (trm : TrmIn)
+--   -- (typ : AST.Typ I)
+-- :=
+--   let inferred := trm.self.infer trm.fuel
+--   let evaled := trm.self.eval trm.fuel
+
+--   -- evaled.map ( fun v =>
+
+--   -- )
+--   -- .getOrElse True
+--   sorry
+--   -- match evaled with
+--   -- | .yields v =>
+--   --   let _inferred : (AST.Trm.val v).infer
+--   --   _inferred <= inferred
+--   -- | .outOfFuel => True
+
+-- -- /--
+-- -- trm with a built-in safety proof
+
+-- -- it's the evaluation target of compile function, like value to eval function
+-- -- -/
+-- -- structure SafeTrm [Compiler.Env I] (I : Free) where
+-- --   trm : AST.Trm I
+-- --   typ : AST.Typ I
+-- --   proof: [Runtime.Env] -> (trm.infer.shouldYields typ) /\   Rec trm.infer.shouldYields typ -- in STLC this is just an equality! extension will happen later
+
+-- -- namespace Proving
+
+-- -- class Env : Type extends Compiler.Env I where
+-- --   proofRefs : FBound I.Index (SafeTrm I)
+
+-- -- end Proving
+
+-- -- -- TODO: mimic Trm.recInfer
+-- -- def proveSafety [fb: FBound I.Index (SafeTrm I)] (trm: AST.Trm I): RecOption (SafeTrm I)
+-- -- | 0 => .outOfFuel
+-- -- | _fule + 1 =>
+-- --   match trm with
+-- --   | .ref k =>
+-- --     -- TODO get AdequateTrm I directly from Compiler Env
+-- --     let v := fb.load (p := ()) k
+-- --     Outcome.yield v
+-- --   | .apply left right => -- TODO: application
+-- --     let _ll := proveSafety left
+-- --     let _rr := proveSafety right
+-- --     ll.typ
+-- --     sorry
+-- --   | .val v =>
+-- --     let condition : Condition I := fun _ => True
+-- --     let proof : trm.CanSatisfy_semi condition := sorry -- TODO trivial, introduce 1 fuel, run Trm.eval immediately and proof CanSatisfy.
+-- --     .mk trm condition proof
+
+-- --     -- argue that _ll must be a function, _rr must be a value of compatible type
+
+-- --     sorry
+
+-- end
+-- end STLC
+
+-- end Lp2lc.Active
